\documentclass{article}
\usepackage{epsfig}
\pagestyle{empty}
\begin{document}
$ \vec x $
\pagebreak

$ \vec u $
\pagebreak

$ f $
\pagebreak

\[ \vec x_k = f \left( x_{k-1}, u_{k-1}, w_{k-1} \right) \]
\pagebreak

$ w $
\pagebreak

$ \vec z $
\pagebreak

\[ \vec z_k = h \left( x_{k-1}, v_{k-1} \right) \]
\pagebreak

$ v $
\pagebreak

\[ \ddot x = \frac{u}{m} - \frac{b_x}{m} \dot x^{2} \]
\pagebreak

\[ \ddot y = \frac{p}{m} \dot x^{2} - g \]
\pagebreak

$ m $
\pagebreak

$ b_{x} $
\pagebreak

$ p $
\pagebreak

$ g $
\pagebreak

$ u $
\pagebreak

\[\vec x_k = \left [ \begin{array}{c} x_k \\ \\ \dot x_k \\ \\ y_k \\ \\ \dot y_k \end{array} \right] = //! \left [ \begin{array}{c} //! x_{k-1} + T \dot x_{k-1} + \frac{T^{2}}{2} \left( \frac{u}{m} - \frac{b_x}{m} \dot x_{k-1}^{2} \right )\\ \\ //! \dot x_{k-1} + T \left ( \frac{u}{m} - \frac{b_x}{m} \dot x_{k-1}^{2} \right ) + w_{1} \\ \\ //! y_{k-1} + T \dot y_{k-1} + \frac{T^{2}}{2} \left( \frac{p}{m} \dot x_{k-1}^{2} - g \right )\\ \\ //! \dot y_{k-1} + T \left( \frac{p}{m} \dot x_{k-1}^{2} - g \right ) + w_{2} //! \end{array} \right ] \]
\pagebreak

$ w_{1} $
\pagebreak

$ w_{2} $
\pagebreak

\[\vec z_k = \left [ \begin{array}{c} \theta \\ \\ r \end{array} \right ] = //! \left [ \begin{array}{c} atan(\frac{y}{x}) +v_{1} \\ \\ \sqrt{x^{2}+y^{2}} + v_{2} \end{array} \right ] \]
\pagebreak

$ v_{1} $
\pagebreak

$ v_{2} $
\pagebreak

\[ A_{[i,j]} = \frac{\partial f_{[i]}}{\partial x_{[j]}} \]
\pagebreak

\[ W_{[i,j]} = \frac{\partial f_{[i]}}{\partial w_{[j]}} \]
\pagebreak

\[ H_{[i,j]} = \frac{\partial h_{[i]}}{\partial x_{[j]}} \]
\pagebreak

\[ V_{[i,j]} = \frac{\partial h_{[i]}}{\partial v_{[j]}} \]
\pagebreak

$ n $
\pagebreak

$ nw $
\pagebreak

$ nv $
\pagebreak

\[ A = \left [ \begin{array}{cccc} //! 1 & T-T^{2} \frac{b}{m} \dot x_{k-1} & 0 & 0 \\ \\ //! 0 & 1-2T \frac{b}{m} \dot x_{k-1} & 0 & 0 \\ \\ //! 0 & T^{2} \frac{p}{m} \dot x_{k-1} & 1 & T \\ \\ //! 0 & 2T \frac{p}{m} \dot x_{k-1} & 0 & 1 //! \end{array} \right ] \]
\pagebreak

\[ W = \left [ \begin{array}{cc} //! 0 & 0 \\ \\ //! 1 & 0 \\ \\ //! 0 & 0\\ \\ //! 0 & 1 //! \end{array} \right ] \]
\pagebreak

\[ H = \left [ \begin{array}{cccc} //! \frac{- \dot y_{k-1}}{x_{k-1}^{2}+y_{k-1}^{2}} & 0 \frac{ \dot x_{k-1}}{x_{k-1}^{2}+y_{k-1}^{2}} & 0 \\ \\ //! \frac{ \dot x_{k-1}}{\sqrt{x_{k-1}^{2}+y_{k-1}^{2}}} & 0 \frac{ \dot y_{k-1}}{\sqrt{x_{k-1}^{2}+y_{k-1}^{2}}} & 0 //! \end{array} \right ] \]
\pagebreak

\[ V = \left [ \begin{array}{cc} //! 1 & 0 \\ \\ //! 0 & 1 //! \end{array} \right ] \]
\pagebreak

\[\vec x = \left [ \begin{array}{c} r\cos\theta \\ 60 \\ r\sin\theta \\ 0 \end{array} \right] \]
\pagebreak

\[ P = \left [ \begin{array}{cccc} //! 100^2 & 0 & 0 & 0 \\ \\ //! 0 & 10^2 & 0 & 0 \\ \\ //! 0 & 0 & 25^2 & 0 \\ \\ //! 0 & 0 & 0 & 10^2 \\ \\ //! \end{array} \right ] \]
\pagebreak

\[ Q = \left [ \begin{array}{cc} //! 0.01^{2} & 0.01^{2}/10 \\ \\ //! 0.01^{2}/10 & 0.01^{2} //! \end{array} \right ] \]
\pagebreak

\[ R = \left [ \begin{array}{cc} //! 0.01^{2} & 0 \\ \\ //! 0 & 0.01^{2} //! \end{array} \right ] \]
\pagebreak

$ h $
\pagebreak

$ x $
\pagebreak

\[ x_k = f \left( x_{k-1}, u_{k-1}, w_{k-1} \right) \]
\pagebreak

\[ Q = E \left( w w^T \right) \]
\pagebreak

$ z $
\pagebreak

\[ z_k = h \left( x_k, v_k \right) \]
\pagebreak

\[ R = E \left( v v^T \right) \]
\pagebreak

$ \hat{x}_{k-1} $
\pagebreak

\[ \tilde{x}_k = f \left( \hat{x}_{k-1}, u_{k-1}, 0 \right) \]
\pagebreak

\[ \tilde{z}_k = h \left( \tilde{x}_k, 0 \right) \]
\pagebreak

$ \tilde{x}_k $
\pagebreak

\[ x_k \approx f \left( \hat{x}_{k-1}, u_{k-1}, 0 \right) //! + \frac{\partial f}{\partial x} \left( \hat{x}_{k-1}, u_{k-1}, 0 \right) //! \left( \Delta x \right) //! + \frac{\partial f}{\partial u} \left( \hat{x}_{k-1}, u_{k-1}, 0 \right) //! \left( \Delta u \right) //! + \frac{\partial f}{\partial w} \left( \hat{x}_{k-1}, u_{k-1}, 0 \right) //! \left( \Delta w \right) \]
\pagebreak

\[ \phantom{x_k} = \tilde{x}_k + A \left( x_{k-1} - \hat{x}_{k-1} //! \right) + W w_{k-1} \]
\pagebreak

\[ z_k \approx h \left( \tilde{x}_k, 0 \right) //! + \frac{\partial h}{\partial x} \left( \tilde{x}_k, 0 \right) //! \left( \Delta x \right) //! + \frac{\partial h}{\partial v} \left( \tilde{x}_k, 0 \right) //! \left( \Delta v \right) \]
\pagebreak

\[ \phantom{z_k} = \tilde{z}_k + H \left( x_k - \tilde{x}_k \right) //! + V v_k \]
\pagebreak

$ f(x, u, 0) $
\pagebreak

$ h(x, 0) $
\pagebreak

$ [-\pi, \pi] $
\pagebreak

\[ Q = E\left( w w^T \right) \]
\pagebreak

\[ R = E\left( v v^T \right) \]
\pagebreak

$ U D U^T $
\pagebreak

$ P = U D U^T $
\pagebreak

$ Q = U_q D_q U_q^T $
\pagebreak

$ = W U_q $
\pagebreak

$ = D_q $
\pagebreak

$ V R V^T $
\pagebreak

$ V R V^T = U_r D_r U_r^T $
\pagebreak

$ ( = D_r ) $
\pagebreak

$ = U_r^{-1} H $
\pagebreak

$ = U_r^{-1} dz $
\pagebreak

$ D_q $
\pagebreak

$ U_q $
\pagebreak

$ \left( U_q^{-1} \right)^T $
\pagebreak

$ nn = n + nw $
\pagebreak

\[ x_k = f \left( x_{k-1}, u_{k-1}, w_{k-1} \right) = //! A x_{k-1} + B u_{k-1} + W w_{k-1} \]
\pagebreak

\[ z_k = h \left( x_k, v_k \right) = //! H x_k + V v_k \]
\pagebreak

\[ \tilde{x}_k = f \left( \hat{x}_{k-1}, u_{k-1}, 0 \right) = //! A \hat{x}_{k-1} + B u_{k-1} \]
\pagebreak

\[ \tilde{z}_k = h \left( \tilde{x}_k, 0 \right) = //! H \tilde{x}_k \]
\pagebreak

\end{document}
